CBS.fst
@@ -4,13 +4,17 @@ open FStar
 open FStar.Seq
 open FStar.HyperStack.ST
 open FStar.Buffer
+open FStar.Mul
+//open FStar.Kremlin.Endianness
 
 module U8 = FStar.UInt8
 module U16 = FStar.UInt16
 module U32 = FStar.UInt32
 
-#set-options "--initial_fuel 0 --max_fuel 0 --z3rlimit 20"
+//#set-options "--initial_fuel 0 --max_fuel 0 --z3rlimit 20"
+#reset-options "--max_fuel 5 --z3rlimit 100"
 
+private
 noeq type cbs_t = | MkCBS: data:(buffer U8.t) -> len:U32.t{U32.v len == length data} -> cbs_t
 
 [@ "substitute"] private
@@ -19,27 +23,91 @@ let u8_to_u32 n = FStar.Int.Cast.uint8_to_uint32 n
 [@ "substitute"] private
 let u32_to_u16 n = FStar.Int.Cast.uint32_to_uint16 n
 
+// TODO move to CBS.Spec
+private
+let rec big_endian (b:seq U8.t) : Tot (n:nat) (decreases (Seq.length b)) =
+  let open FStar.Seq in
+    if length b = 0 then 0
+    else U8.v (last b) + pow2 8 * big_endian (slice b 0 (length b - 1))
+
+(*
+private
+val big_endian_single: n:U8.t -> Lemma
+  (ensures (big_endian (Seq.create 1 n) = U8.v n))
+  [SMTPat (big_endian (Seq.create 1 n) = U8.v n)]
+let big_endian_single n =
+  let open FStar.Seq in
+  let s = (create 1 n) in
+  assert (big_endian s = U8.v (index s 0) + pow2 8 * big_endian (slice s 0 0));
+  assert (U8.v (index s 0) > 0 ==> big_endian s > 0);
+  assert (big_endian s > 0 ==> U8.v (index s 0) > 0);
+  assert (U8.v (index s 0) = 0 ==> big_endian s = 0);
+  assert (big_endian s = 0 ==> U8.v (index s 0) = 0);
+  ()
+*)
+
+private
+let lemma_uint32s_from_le_def_0 (b:seq U8.t{Seq.length b == 0}) : Lemma
+  (big_endian b == 0)
+= ()
+
 val cbs_get_u :
   cbs: buffer cbs_t{length cbs = 1} ->
   out: buffer U32.t{length out = 1} ->
   num: U32.t{U32.(v num > 0 /\ v num < 5)} ->
   ST bool
   (requires (fun h -> live h out /\ live h cbs /\ live h (get h cbs 0).data))
-  (ensures (fun h0 r h1 -> live h1 out)) // (not(r) \/ modifies_1 out h0 h1) ?
-  // TODO check resulting *out
+  (ensures (fun h0 r h1 -> live h1 out /\ // modifies_1 out h0 h1 ?
+    (let cbs0 = get h0 cbs 0 in
+      // Return false if there aren't enough bytes.
+      r == U32.(v cbs0.len >= v num) //\
+      // If there are, check the result.
+      //(not(r) \/ U32.v (get h1 out 0) == big_endian (slice (as_seq h0 cbs0.data) 0 (U32.v num)))
+      //(not(r) \/ U32.v (get h1 out 0) == be_to_n (as_seq h0 cbs0.data))
+      //(not(r) \/ U32.v (get h1 out 0) == be_to_n (slice (as_seq h0 cbs0.data) 0 (U32.v num)))
+    )))
 
 let cbs_get_u cbs out num =
+  //out.(0ul) <- 0ul;
   let cbs0 = cbs.(0ul) in
   if U32.(cbs0.len >=^ num) then (
-    let inv = (fun h _ -> live h out /\ live h cbs0.data) in
+    let inv = (fun h _ -> live h out /\ live h cbs0.data
+      ///\ U32.v (get h out 0) == big_endian (slice (as_seq h cbs0.data) 0 i)) in
+      ///\ U32.v (get h out 0) == be_to_n (slice (as_seq h cbs0.data) 0 i)
+      ///\ Seq.length (slice (as_seq h cbs0.data) 0 0) == 0
+      ///\ be_to_n (Seq.create 0 0uy) == 0
+      ///\ big_endian (Seq.create 0 0uy) == 0
+      ///\ big_endian (slice (as_seq h cbs0.data) 0 0) == 0
+      ///\ big_endian (slice (as_seq h cbs0.data) 0 0) == 0
+    ) in
     let f (i:U32.t{U32.(v 0ul <= v i /\ v i < v num)}) :
       Stack unit
         (requires (fun h -> live h out /\ live h cbs0.data))
         (ensures (fun h0 _ h1 -> modifies_1 out h0 h1))
       = let bi = cbs0.data.(i) in
-        out.(0ul) <- U32.((out.(0ul) <<^ 8ul) +^ u8_to_u32 bi)
+        let lo = u8_to_u32 bi in
+      //Math.Lemmas.pow2_lt_compat 32 8; // TODO
+      //cut (U32.v lo = U8.v bi); // TODO
+      //Math.Lemmas.pow2_lt_compat 16 8;
+      //Math.Lemmas.pow2_lt_compat 24 16;
+      //Math.Lemmas.pow2_lt_compat 32 24;
+      //Math.Lemmas.pow2_plus 8 8;
+      //Math.Lemmas.pow2_plus 8 16;
+      //Math.Lemmas.pow2_plus 8 24;
+        let hi = U32.(out.(0ul) <<^ 8ul) in
+      //UInt.shift_left_value_lemma #32 (U32.v out.(0ul)) 8;
+      //Math.Lemmas.modulo_lemma (U32.v out.(0ul)) (pow2 32);
+      //Math.Lemmas.modulo_lemma (U32.v hi) (pow2 32); // TODO
+      //cut (U32.v hi == (pow2 8) * (U32.v out.(0ul)));
+        let res = U32.(hi |^ lo) in
+      //UInt.logor_disjoint #32 (U32.v hi) (U32.v lo) 8;
+      //assert (U32.v res == (U32.v hi) + (U32.v lo));
+      //assert U32.(v res == v lo + v out.(0ul) * (pow2 8)); // TODO
+        out.(0ul) <- res
     in
     C.Loops.for 0ul num inv f;
+    //let h = FStar.HyperStack.ST.get () in
+    //assert (U32.v out.(0ul) == big_endian (slice (as_seq h cbs0.data) 0 (U32.v num)));
     true
   ) else (
     false
@@ -55,7 +123,8 @@ val cbs_get_u8 :
       // Return false if there aren't enough bytes.
       r == (U32.v cbs0.len > 0) /\
       // If there are, the result will be cbs->data[0].
-      (not(r) \/ get h1 out 0 == get h0 cbs0.data 0)
+      //(not(r) \/ get h1 out 0 == get h0 cbs0.data 0) // TODO
+      (not(r) \/ U8.v (get h1 out 0) == big_endian (slice (as_seq h0 cbs0.data) 0 1))
     )))
 
 let cbs_get_u8 cbs out =
